Get CEK to evaluate lists

src/Exp.v
@@ -1,6 +1,7 @@
 Require Export
   Ty
   Lit
+  ilist
   Coq.Lists.List.
 
 From Equations Require Import Equations.
@@ -21,8 +22,7 @@ Derive Signature NoConfusion for Var.
 Inductive Exp Γ : Ty → Type :=
   | Constant {ty} : Literal ty → Exp Γ (TyPrim ty)
   | Seq {τ τ'}    : Exp Γ τ' → Exp Γ τ → Exp Γ τ
-  (* | Nil {τ}       : Exp Γ (TyList τ) *)
-  (* | Cons {τ}      : Exp Γ τ → Exp Γ (TyList τ) → Exp Γ (TyList τ) *)
+  | List {τ}      : list (Exp Γ τ) → Exp Γ (TyList τ)
   | Let {τ ty}    : Exp Γ ty → Exp (ty :: Γ) τ → Exp Γ τ
 
   (* These are the terms of the base lambda calculus *)
@@ -32,6 +32,40 @@ Inductive Exp Γ : Ty → Type :=
 
 Derive Signature for Exp.
 
+Variable P : ∀ Γ τ, Exp Γ τ → Type.
+
+Variable Pconstant : ∀ Γ ty (lit : Literal ty),
+  P Γ (TyPrim ty) (Constant Γ lit).
+Variable Pseq      : ∀ Γ τ τ' (e1 : Exp Γ τ') (e2 : Exp Γ τ),
+  P Γ τ' e1 → P Γ τ e2 → P Γ τ (Seq Γ e1 e2).
+Variable Plist     : ∀ Γ τ l,
+  ilist (P Γ τ) l → P Γ (TyList τ) (List Γ l).
+Variable Plet      : ∀ Γ τ ty (x : Exp Γ ty) (body : Exp (ty :: Γ) τ),
+  P Γ ty x →
+  P (ty :: Γ) τ body →
+  P Γ τ (Let _ x body).
+Variable Pvar      : ∀ Γ τ (v : Var Γ τ),
+  P Γ τ (VAR Γ v).
+Variable Plam      : ∀ Γ dom cod (e : Exp (dom :: Γ) cod),
+  P (dom :: Γ) cod e → P Γ (dom ⟶ cod) (LAM Γ e).
+Variable Papp      : ∀ Γ dom cod (e1 : Exp Γ (dom ⟶ cod)) (e2 : Exp Γ dom),
+  P Γ (dom ⟶ cod) e1 →
+  P Γ dom e2 →
+  P Γ cod (APP Γ e1 e2).
+
+Equations Exp_rect' {Γ τ} (e : Exp Γ τ) : P Γ τ e :=
+  Exp_rect' (Constant _ lit) := Pconstant _ _ lit;
+  Exp_rect' (Seq _ e1 e2)    := Pseq _ _ _ _ _ (Exp_rect' e1) (Exp_rect' e2);
+  Exp_rect' (List _ l)       := Plist _ _ _ (Exp_sub_rect' l);
+  Exp_rect' (Let _ x body)   := Plet _ _ _ _ _ (Exp_rect' x) (Exp_rect' body);
+  Exp_rect' (VAR _ v)        := Pvar _ _ v;
+  Exp_rect' (LAM _ e)        := Plam _ _ _ _ (Exp_rect' e);
+  Exp_rect' (APP _ e1 e2)    := Papp _ _ _ _ _ (Exp_rect' e1) (Exp_rect' e2);
+
+where Exp_sub_rect' {Γ τ} (l : list (Exp Γ τ)) : ilist (P Γ τ) l :=
+  Exp_sub_rect' [] := tt;
+  Exp_sub_rect' (x :: xs) := (Exp_rect' x, Exp_sub_rect' xs).
+
 End Exp.
 
 Arguments ZV {_ _}.
@@ -39,8 +73,7 @@ Arguments SV {_ _ _} _.
 
 Arguments Constant {Γ ty} _.
 Arguments Seq {Γ τ τ'} _ _.
-(* Arguments Nil {Γ τ}. *)
-(* Arguments Cons {Γ τ} _ _. *)
+Arguments List {Γ τ} _.
 Arguments Let {Γ τ ty} _ _.
 Arguments VAR {Γ τ} _.
 Arguments LAM {Γ dom cod} _.
