src/ilist.v
@@ -1,0 +1,11 @@
+Require Import
+  Coq.Unicode.Utf8
+  Coq.Lists.List.
+
+Import ListNotations.
+
+Fixpoint ilist {A} (B : A → Type) (l : list A) : Type :=
+  match l with
+  | []      => unit
+  | x :: xs => B x * ilist B xs
+  end.
